theories/zoo/program_logic/prophet_wise.v
@@ -14,252 +14,14 @@ From zoo.diaframe Require Import
 From zoo Require Import
   options.
 
-Class ProphetWiseStrongG Σ `{zoo_G : !ZooG Σ} prophet :=
-  { #[local] prophet_wise_strong_G_full_G :: AgreeG Σ (leibnizO (list prophet.(prophet_typed_strong_type)))
-  ; #[local] prophet_wise_strong_G_past_G :: MonoListG Σ prophet.(prophet_typed_strong_type)
-  }.
-
-Definition prophet_wise_strong_Σ prophet :=
-  #[agree_Σ (leibnizO (list prophet.(prophet_typed_strong_type)))
-  ; mono_list_Σ prophet.(prophet_typed_strong_type)
-  ].
-#[global] Instance subG_prophet_wise_strong_Σ Σ `{zoo_G : !ZooG Σ} prophet :
-  subG (prophet_wise_strong_Σ prophet) Σ →
-  ProphetWiseStrongG Σ prophet.
-Proof.
-  solve_inG.
-Qed.
-
-Section prophet_wise_strong_G.
-  Context (prophet : prophet_typed_strong).
-  Context `{prophet_wise_strong_G : ProphetWiseStrongG Σ prophet}.
-
-  Implicit Types proph : prophet.(prophet_typed_strong_type).
-  Implicit Types prophs : list prophet.(prophet_typed_strong_type).
-
-  Record prophet_wise_strong_name :=
-    { prophet_wise_strong_name_full : gname
-    ; prophet_wise_strong_name_past : gname
-    }.
-
-  #[global] Instance prophet_wise_strong_name_eq_dec : EqDecision prophet_wise_strong_name :=
-    ltac:(solve_decision).
-  #[global] Instance prophet_wise_strong_name_countable :
-    Countable prophet_wise_strong_name.
-  Proof.
-    solve_countable.
-  Qed.
-
-  Definition prophet_wise_strong_full γ prophs :=
-    agree_on γ.(prophet_wise_strong_name_full) prophs.
-  #[local] Instance : CustomIpat "full" :=
-    " #Hfull{}
-    ".
-
-  Definition prophet_wise_strong_model pid γ past prophs : iProp Σ :=
-    prophet_wise_strong_full γ (past ++ prophs) ∗
-    mono_list_auth γ.(prophet_wise_strong_name_past) (DfracOwn 1) past ∗
-    prophet_typed_strong_model prophet pid prophs.
-  #[local] Instance : CustomIpat "model" :=
-    " ( #Hfull{}
-      & Hpast{}_auth
-      & Hmodel{}
-      )
-    ".
-
-  Definition prophet_wise_strong_snapshot γ past prophs : iProp Σ :=
-    prophet_wise_strong_full γ (past ++ prophs) ∗
-    mono_list_lb γ.(prophet_wise_strong_name_past) past.
-  #[local] Instance : CustomIpat "snapshot" :=
-    " ( #Hfull{suff}
-      & #Hpast_lb
-      )
-    ".
-
-  Definition prophet_wise_strong_lb γ lb : iProp Σ :=
-    ∃ past,
-    prophet_wise_strong_snapshot γ past lb.
-  #[local] Instance : CustomIpat "lb" :=
-    " ( %past{suff}
-      & Hsnapshot
-      )
-    ".
-
-  #[global] Instance prophet_wise_strong_full_timeless γ prophs :
-    Timeless (prophet_wise_strong_full γ prophs).
-  Proof.
-    apply _.
-  Qed.
-  #[global] Instance prophet_wise_strong_model_timeless pid γ past prophs :
-    Timeless (prophet_wise_strong_model pid γ past prophs).
-  Proof.
-    apply _.
-  Qed.
-  #[global] Instance prophet_wise_strong_snapshot_timeless γ past prophs :
-    Timeless (prophet_wise_strong_snapshot γ past prophs).
-  Proof.
-    apply _.
-  Qed.
-  #[global] Instance prophet_wise_strong_lb_timeless γ lb :
-    Timeless (prophet_wise_strong_lb γ lb).
-  Proof.
-    apply _.
-  Qed.
-
-  #[global] Instance prophet_wise_strong_full_persistent γ prophs :
-    Persistent (prophet_wise_strong_full γ prophs).
-  Proof.
-    apply _.
-  Qed.
-  #[global] Instance prophet_wise_strong_snapshot_persistent γ past prophs :
-    Persistent (prophet_wise_strong_snapshot γ past prophs).
-  Proof.
-    apply _.
-  Qed.
-  #[global] Instance prophet_wise_strong_lb_persistent γ lb :
-    Persistent (prophet_wise_strong_lb γ lb).
-  Proof.
-    apply _.
-  Qed.
-
-  Lemma prophet_wise_strong_model_exclusive pid γ1 past1 prophs1 γ2 past2 prophs2 :
-    prophet_wise_strong_model pid γ1 past1 prophs1 -∗
-    prophet_wise_strong_model pid γ2 past2 prophs2 -∗
-    False.
-  Proof.
-    iIntros "(:model =1) (:model =2)".
-    iApply (prophet_typed_strong_model_exclusive with "Hmodel1 Hmodel2").
-  Qed.
-
-  Lemma prophet_wise_strong_full_get pid γ past prophs :
-    prophet_wise_strong_model pid γ past prophs ⊢
-    prophet_wise_strong_full γ (past ++ prophs).
-  Proof.
-    iSteps.
-  Qed.
-  Lemma prophet_wise_strong_full_get' pid γ past prophs :
-    prophet_wise_strong_model pid γ past prophs ⊢
-      ∃ prophs',
-      prophet_wise_strong_full γ prophs'.
-  Proof.
-    rewrite prophet_wise_strong_full_get. iSteps.
-  Qed.
-  Lemma prophet_wise_strong_full_valid pid γ past prophs1 prophs2 :
-    prophet_wise_strong_model pid γ past prophs1 -∗
-    prophet_wise_strong_full γ prophs2 -∗
-    ⌜prophs2 = past ++ prophs1⌝.
-  Proof.
-    iIntros "(:model =1) (:full =2)".
-    iDestruct (agree_on_agree_L with "Hfull1 Hfull2") as %<-.
-    iSteps.
-  Qed.
-  Lemma prophet_wise_strong_full_agree γ prophs1 prophs2 :
-    prophet_wise_strong_full γ prophs1 -∗
-    prophet_wise_strong_full γ prophs2 -∗
-    ⌜prophs1 = prophs2⌝.
-  Proof.
-    apply: agree_on_agree_L.
-  Qed.
-
-  Lemma prophet_wise_strong_snapshot_get pid γ past prophs :
-    prophet_wise_strong_model pid γ past prophs ⊢
-    prophet_wise_strong_snapshot γ past prophs.
-  Proof.
-    iIntros "(:model)".
-    iStep.
-    iApply (mono_list_lb_get with "Hpast_auth").
-  Qed.
-  Lemma prophet_wise_strong_snapshot_valid pid γ past1 prophs1 past2 prophs2 :
-    prophet_wise_strong_model pid γ past1 prophs1 -∗
-    prophet_wise_strong_snapshot γ past2 prophs2 -∗
-      ∃ past3,
-      ⌜past1 = past2 ++ past3⌝ ∗
-      ⌜prophs2 = past3 ++ prophs1⌝.
-  Proof.
-    iIntros "(:model) (:snapshot suff=')".
-    iDestruct (agree_on_agree_L with "Hfull Hfull'") as %Hfull.
-    iDestruct (mono_list_lb_valid with "Hpast_auth Hpast_lb") as %(past3 & ->).
-    iPureIntro. rewrite -assoc in Hfull. naive_solver.
-  Qed.
-
-  Lemma prophet_wise_strong_lb_get pid γ past prophs :
-    prophet_wise_strong_model pid γ past prophs ⊢
-    prophet_wise_strong_lb γ prophs.
-  Proof.
-    rewrite prophet_wise_strong_snapshot_get.
-    iSteps.
-  Qed.
-  Lemma prophet_wise_strong_lb_valid pid γ past prophs lb :
-    prophet_wise_strong_model pid γ past prophs -∗
-    prophet_wise_strong_lb γ lb -∗
-      ∃ past1 past2,
-      ⌜past = past1 ++ past2⌝ ∗
-      ⌜lb = past2 ++ prophs⌝.
-  Proof.
-    iIntros "Hmodel (:lb suff=')".
-    iExists past'.
-    iApply (prophet_wise_strong_snapshot_valid with "Hmodel Hsnapshot").
-  Qed.
-
-  Lemma prophet_wise_strong_wp_proph E :
-    {{{
-      True
-    }}}
-      Proph @ E
-    {{{
-      pid γ prophs
-    , RET #pid;
-      prophet_wise_strong_model pid γ [] prophs
-    }}}.
-  Proof.
-    iIntros "%Φ _ HΦ".
-    iApply wp_fupd. wp_apply (prophet_typed_strong_wp_proph with "[//]") as "%pid %prophs Hpid".
-    iMod (agree_alloc (agree_G := prophet_wise_strong_G_full_G) prophs) as "(%γ_full & #Hfull)".
-    iMod (mono_list_alloc []) as "(%γ_past & Hpast_auth)".
-    set γ :=
-      {|prophet_wise_strong_name_full := γ_full
-      ; prophet_wise_strong_name_past := γ_past
-      |}.
-    iApply ("HΦ" $! pid γ).
-    iSteps.
-  Qed.
-
-  Lemma prophet_wise_strong_wp_resolve e pid v γ past prophs E Φ :
-    Atomic e →
-    to_val e = None →
-    prophet_wise_strong_model pid γ past prophs -∗
-    WP e @ E {{ w,
-      ∃ proph,
-      ⌜prophet.(prophet_typed_strong_of_val) w v = Some proph⌝ ∗
-        ∀ prophs',
-        ⌜prophs = proph :: prophs'⌝ -∗
-        prophet_wise_strong_model pid γ (past ++ [proph]) prophs' -∗
-        Φ w
-    }} -∗
-    WP Resolve e #pid v @ E {{ Φ }}.
-  Proof.
-    iIntros "% % (:model) HΦ".
-    wp_apply (prophet_typed_strong_wp_resolve with "Hmodel"); first done.
-    iApply wp_fupd. wp_apply (wp_wand with "HΦ") as "%w (%proph & % & HΦ)".
-    iExists proph. iSplitR; first done.
-    iMod (mono_list_update_snoc proph with "Hpast_auth") as "Hpast_auth".
-    iIntros "!> %prophs' -> Hpid".
-    iApply ("HΦ" with "[//]").
-    rewrite (assoc _ _ [_]). iSteps.
-  Qed.
-End prophet_wise_strong_G.
-
-#[global] Opaque prophet_wise_strong_full.
-#[global] Opaque prophet_wise_strong_model.
-#[global] Opaque prophet_wise_strong_snapshot.
-#[global] Opaque prophet_wise_strong_lb.
-
 Class ProphetWiseG Σ `{zoo_G : !ZooG Σ} prophet :=
-  { #[local] prophet_wise_G :: ProphetWiseStrongG Σ prophet
+  { #[local] prophet_wise_G_full_G :: AgreeG Σ (leibnizO (list prophet.(prophet_typed_type)))
+  ; #[local] prophet_wise_G_past_G :: MonoListG Σ prophet.(prophet_typed_type)
   }.
 
 Definition prophet_wise_Σ prophet :=
-  #[prophet_wise_strong_Σ prophet
+  #[agree_Σ (leibnizO (list prophet.(prophet_typed_type)))
+  ; mono_list_Σ prophet.(prophet_typed_type)
   ].
 #[global] Instance subG_prophet_wise_Σ Σ `{zoo_G : !ZooG Σ} prophet :
   subG (prophet_wise_Σ prophet) Σ →
@@ -273,27 +35,53 @@ Section prophet_wise_G.
   Context `{prophet_wise_G : ProphetWiseG Σ prophet}.
 
   Implicit Types proph : prophet.(prophet_typed_type).
-  Implicit Types past prophs lb : list prophet.(prophet_typed_type).
+  Implicit Types prophs : list prophet.(prophet_typed_type).
 
-  Definition prophet_wise_name :=
-    prophet_wise_strong_name.
-  Implicit Types γ : prophet_wise_name.
+  Record prophet_wise_name :=
+    { prophet_wise_name_full : gname
+    ; prophet_wise_name_past : gname
+    }.
+
+  #[global] Instance prophet_wise_name_eq_dec : EqDecision prophet_wise_name :=
+    ltac:(solve_decision).
+  #[global] Instance prophet_wise_name_countable :
+    Countable prophet_wise_name.
+  Proof.
+    solve_countable.
+  Qed.
 
   Definition prophet_wise_full γ prophs :=
-    prophet_wise_strong_full prophet γ prophs.
+    agree_on γ.(prophet_wise_name_full) prophs.
+  #[local] Instance : CustomIpat "full" :=
+    " #Hfull{}
+    ".
 
-  Definition prophet_wise_model pid γ past prophs :=
-    prophet_wise_strong_model prophet pid γ past prophs.
+  Definition prophet_wise_model pid γ past prophs : iProp Σ :=
+    prophet_wise_full γ (past ++ prophs) ∗
+    mono_list_auth γ.(prophet_wise_name_past) (DfracOwn 1) past ∗
+    prophet_typed_model prophet pid prophs.
+  #[local] Instance : CustomIpat "model" :=
+    " ( #Hfull{}
+      & Hpast{}_auth
+      & Hmodel{}
+      )
+    ".
 
-  Definition prophet_wise_snapshot γ past prophs :=
-    prophet_wise_strong_snapshot prophet γ past prophs.
+  Definition prophet_wise_snapshot γ past prophs : iProp Σ :=
+    prophet_wise_full γ (past ++ prophs) ∗
+    mono_list_lb γ.(prophet_wise_name_past) past.
+  #[local] Instance : CustomIpat "snapshot" :=
+    " ( #Hfull{suff}
+      & #Hpast_lb
+      )
+    ".
 
-  Definition prophet_wise_lb γ lb :=
-    prophet_wise_strong_lb prophet γ lb.
+  Definition prophet_wise_lb γ lb : iProp Σ :=
+    ∃ past,
+    prophet_wise_snapshot γ past lb.
   #[local] Instance : CustomIpat "lb" :=
-    " ( %slb
-      & ->
-      & Hlb
+    " ( %past{suff}
+      & Hsnapshot
       )
     ".
 
@@ -317,6 +105,7 @@ Section prophet_wise_G.
   Proof.
     apply _.
   Qed.
+
   #[global] Instance prophet_wise_full_persistent γ prophs :
     Persistent (prophet_wise_full γ prophs).
   Proof.
@@ -338,14 +127,15 @@ Section prophet_wise_G.
     prophet_wise_model pid γ2 past2 prophs2 -∗
     False.
   Proof.
-    apply prophet_wise_strong_model_exclusive.
+    iIntros "(:model =1) (:model =2)".
+    iApply (prophet_typed_model_exclusive with "Hmodel1 Hmodel2").
   Qed.
 
   Lemma prophet_wise_full_get pid γ past prophs :
     prophet_wise_model pid γ past prophs ⊢
     prophet_wise_full γ (past ++ prophs).
   Proof.
-    apply prophet_wise_strong_full_get.
+    iSteps.
   Qed.
   Lemma prophet_wise_full_get' pid γ past prophs :
     prophet_wise_model pid γ past prophs ⊢
@@ -359,21 +149,25 @@ Section prophet_wise_G.
     prophet_wise_full γ prophs2 -∗
     ⌜prophs2 = past ++ prophs1⌝.
   Proof.
-    apply prophet_wise_strong_full_valid.
+    iIntros "(:model =1) (:full =2)".
+    iDestruct (agree_on_agree_L with "Hfull1 Hfull2") as %<-.
+    iSteps.
   Qed.
   Lemma prophet_wise_full_agree γ prophs1 prophs2 :
     prophet_wise_full γ prophs1 -∗
     prophet_wise_full γ prophs2 -∗
     ⌜prophs1 = prophs2⌝.
   Proof.
-    apply prophet_wise_strong_full_agree.
+    apply: agree_on_agree_L.
   Qed.
 
   Lemma prophet_wise_snapshot_get pid γ past prophs :
     prophet_wise_model pid γ past prophs ⊢
     prophet_wise_snapshot γ past prophs.
   Proof.
-    apply prophet_wise_strong_snapshot_get.
+    iIntros "(:model)".
+    iStep.
+    iApply (mono_list_lb_get with "Hpast_auth").
   Qed.
   Lemma prophet_wise_snapshot_valid pid γ past1 prophs1 past2 prophs2 :
     prophet_wise_model pid γ past1 prophs1 -∗
@@ -382,14 +176,18 @@ Section prophet_wise_G.
       ⌜past1 = past2 ++ past3⌝ ∗
       ⌜prophs2 = past3 ++ prophs1⌝.
   Proof.
-    apply prophet_wise_strong_snapshot_valid.
+    iIntros "(:model) (:snapshot suff=')".
+    iDestruct (agree_on_agree_L with "Hfull Hfull'") as %Hfull.
+    iDestruct (mono_list_lb_valid with "Hpast_auth Hpast_lb") as %(past3 & ->).
+    iPureIntro. rewrite -assoc in Hfull. naive_solver.
   Qed.
 
   Lemma prophet_wise_lb_get pid γ past prophs :
-    prophet_wise_model pid γ past prophs -∗
+    prophet_wise_model pid γ past prophs ⊢
     prophet_wise_lb γ prophs.
   Proof.
-    iApply prophet_wise_strong_lb_get.
+    rewrite prophet_wise_snapshot_get.
+    iSteps.
   Qed.
   Lemma prophet_wise_lb_valid pid γ past prophs lb :
     prophet_wise_model pid γ past prophs -∗
@@ -398,7 +196,9 @@ Section prophet_wise_G.
       ⌜past = past1 ++ past2⌝ ∗
       ⌜lb = past2 ++ prophs⌝.
   Proof.
-    apply prophet_wise_strong_lb_valid.
+    iIntros "Hmodel (:lb suff=')".
+    iExists past'.
+    iApply (prophet_wise_snapshot_valid with "Hmodel Hsnapshot").
   Qed.
 
   Lemma prophet_wise_wp_proph E :
@@ -412,29 +212,43 @@ Section prophet_wise_G.
       prophet_wise_model pid γ [] prophs
     }}}.
   Proof.
-    apply: prophet_wise_strong_wp_proph.
+    iIntros "%Φ _ HΦ".
+    iApply wp_fupd. wp_apply (prophet_typed_wp_proph with "[//]") as "%pid %prophs Hpid".
+    iMod (agree_alloc (agree_G := prophet_wise_G_full_G) prophs) as "(%γ_full & #Hfull)".
+    iMod (mono_list_alloc []) as "(%γ_past & Hpast_auth)".
+    set γ :=
+      {|prophet_wise_name_full := γ_full
+      ; prophet_wise_name_past := γ_past
+      |}.
+    iApply ("HΦ" $! pid γ).
+    iSteps.
   Qed.
 
-  Lemma prophet_wise_wp_resolve proph e pid v γ past prophs E Φ :
+  Lemma prophet_wise_wp_resolve e pid v γ past prophs E Φ :
     Atomic e →
     to_val e = None →
-    prophet.(prophet_typed_of_val) v = Some proph →
     prophet_wise_model pid γ past prophs -∗
     WP e @ E {{ w,
-      ∀ prophs',
-      ⌜prophs = proph :: prophs'⌝ -∗
-      prophet_wise_model pid γ (past ++ [proph]) prophs' -∗
-      Φ w
+      ∃ proph,
+      ⌜prophet.(prophet_typed_of_val) w v = Some proph⌝ ∗
+        ∀ prophs',
+        ⌜prophs = proph :: prophs'⌝ -∗
+        prophet_wise_model pid γ (past ++ [proph]) prophs' -∗
+        Φ w
     }} -∗
     WP Resolve e #pid v @ E {{ Φ }}.
   Proof.
-    iIntros (? ? Hproph) "Hmodel HΦ".
-    wp_apply (prophet_wise_strong_wp_resolve with "Hmodel"); first done.
-    iSteps.
+    iIntros "% % (:model) HΦ".
+    wp_apply (prophet_typed_wp_resolve with "Hmodel"); first done.
+    iApply wp_fupd. wp_apply (wp_wand with "HΦ") as "%w (%proph & % & HΦ)".
+    iExists proph. iSplitR; first done.
+    iMod (mono_list_update_snoc proph with "Hpast_auth") as "Hpast_auth".
+    iIntros "!> %prophs' -> Hpid".
+    iApply ("HΦ" with "[//]").
+    rewrite (assoc _ _ [_]). iSteps.
   Qed.
 End prophet_wise_G.
 
-#[global] Opaque prophet_wise_name.
 #[global] Opaque prophet_wise_full.
 #[global] Opaque prophet_wise_model.
 #[global] Opaque prophet_wise_snapshot.
