theories/zoo_saturn/mpmc_bqueue.v
@@ -40,9 +40,9 @@ Implicit Types waiter : gname.
 Implicit Types waiters : gmap gname nat.
 
 #[local] Definition prophet :=
-  {|prophet_typed_strong_1_type :=
+  {|prophet_typed_1_type :=
       location
-  ; prophet_typed_strong_1_of_val v _ :=
+  ; prophet_typed_1_of_val v _ :=
       match v with
       | ValLoc l =>
           Some l
@@ -878,7 +878,7 @@ Module base.
       wp_rec.
       wp_apply (front𑁒spec with "Hinv") as (front1 i_front1) "(:node_model =front1 front=)".
       wp_match.
-      wp_apply+ (prophet_typed_strong_1_wp_proph prophet with "[//]") as (pid proph) "Hproph".
+      wp_apply+ (prophet_typed_1_wp_proph prophet with "[//]") as (pid proph) "Hproph".
       wp_apply+ (back𑁒spec with "Hinv") as (back2 i_back2) "(:node_model =back2)".
       wp_match. wp_pures.
       destruct_decide (proph = front1) as -> | Hproph.
@@ -889,7 +889,7 @@ Module base.
 
           wp_bind (Resolve _ _ _).
           iInv "Hinv" as "(:inv_inner =3)".
-          wp_apply (prophet_typed_strong_1_wp_resolve with "Hproph"); first done.
+          wp_apply (prophet_typed_1_wp_resolve with "Hproph"); first done.
           wp_load.
           iStep. iIntros "<-".
           iDestruct "HΦ" as "[HΦ | (%i_front2 & #Hfront_lb_front2 & % & HΦ)]"; last first.
@@ -919,7 +919,7 @@ Module base.
 
           wp_bind (Resolve _ _ _).
           iInv "Hinv" as "(:inv_inner =3)".
-          wp_apply (prophet_typed_strong_1_wp_resolve with "Hproph"); first done.
+          wp_apply (prophet_typed_1_wp_resolve with "Hproph"); first done.
           iSteps.
 
         + wp_match. wp_pures.
