theories/zoo/program_logic/prophet_bool.v
@@ -10,7 +10,7 @@ From zoo Require Import
 Definition prophet_bool :=
   {|prophet_typed_type :=
       bool
-  ; prophet_typed_of_val v :=
+  ; prophet_typed_of_val _ v :=
       match v with
       | ValBool b =>
           Some b
@@ -22,7 +22,7 @@ Definition prophet_bool :=
 Definition prophet_bool_1 :=
   {|prophet_typed_1_type :=
       bool
-  ; prophet_typed_1_of_val v :=
+  ; prophet_typed_1_of_val _ v :=
       match v with
       | ValBool b =>
           Some b
