theories/zoo_saturn/inf_ws_deque_1.v
@@ -1211,9 +1211,9 @@ Module base.
 
       iInv "Hinv" as "(:inv_inner =3)".
       iDestruct (front_lb_valid with "Hfront_auth Hfront_lb") as %?.
-      wp_apply (prophet_multi_wp_resolve' with "Hprophet_model"); [done.. |].
+      wp_apply (prophet_multi_wp_resolve' with "Hprophet_model"). 1: done.
       wp_cas as Hcas; zoo_simplify in Hcas; last lia.
-      iIntros "!> %prophs %Hprophss3 Hprophet_model".
+      iStep. iIntros "%prophs %Hprophss3 Hprophet_model".
       iSplitR "HΦ".
       { iFrameSteps.
         - iPureIntro => *.
@@ -1240,9 +1240,9 @@ Module base.
 
       iInv "Hinv" as "(:inv_inner =1)".
       iDestruct (front_lb_valid with "Hfront_auth Hfront_lb") as %?.
-      wp_apply (prophet_multi_wp_resolve' with "Hprophet_model"); [done.. |].
+      wp_apply (prophet_multi_wp_resolve' with "Hprophet_model"). 1: done.
       wp_apply (wp_cas_nobranch' with "Ht_front") as (b) "%Hcas Ht_front".
-      iIntros "%prophs %Hprophss1 Hprophet_model".
+      iStep. iIntros "%prophs %Hprophss1 Hprophet_model".
       destruct b; zoo_simplify in Hcas; first subst front1.
 
       - iDestruct (prophet_multi_full_valid with "Hprophet_model Hprophet_full") as %->.
@@ -1273,9 +1273,9 @@ Module base.
       iIntros "%Φ ((:inv') & Hwinner_pop) HΦ".
 
       iInv "Hinv" as "(:inv_inner =1)".
-      wp_apply (prophet_multi_wp_resolve' with "Hprophet_model"); [done.. |].
+      wp_apply (prophet_multi_wp_resolve' with "Hprophet_model"). 1: done.
       wp_apply (wp_cas_nobranch' with "Ht_front") as (b) "%Hcas Ht_front".
-      iIntros "%prophs %Hprophss1 Hprophet_model".
+      iStep. iIntros "%prophs %Hprophss1 Hprophet_model".
       iDestruct (inv_state_winner_pop with "Hstate Hwinner_pop") as "(%P_ & -> & #Heq & Hstate & Hwinner_pop)".
       rewrite Hprophss1.
       destruct b; zoo_simplify in Hcas; last congruence.
@@ -1340,9 +1340,9 @@ Module base.
       iIntros "%Φ ((:inv') & Hwinner_steal) HΦ".
 
       iInv "Hinv" as "(:inv_inner =1)".
-      wp_apply (prophet_multi_wp_resolve' with "Hprophet_model"); [done.. |].
+      wp_apply (prophet_multi_wp_resolve' with "Hprophet_model"). 1: done.
       wp_apply (wp_cas_nobranch' with "Ht_front") as (b) "%Hcas Ht_front".
-      iIntros "%prophs %Hprophss1 Hprophet_model".
+      iStep. iIntros "%prophs %Hprophss1 Hprophet_model".
       iDestruct (inv_state_winner_steal with "Hstate Hwinner_steal") as "(%P_ & -> & _ & (:inv_state_emptyish_pop =1) & Hwinner_steal)".
       destruct b; zoo_simplify in Hcas; last congruence.
       iMod (front_update with "Hfront_auth") as "Hfront_auth".
@@ -1372,9 +1372,9 @@ Module base.
       iIntros "%Φ ((:inv') & Howner₁ & #Hfront_lb) HΦ".
 
       iInv "Hinv" as "(:inv_inner =1)".
-      wp_apply (prophet_multi_wp_resolve' with "Hprophet_model"); [done.. |].
+      wp_apply (prophet_multi_wp_resolve' with "Hprophet_model"). 1: done.
       wp_apply (wp_cas_nobranch' with "Ht_front") as (b) "%Hcas Ht_front".
-      iIntros "%prophs %Hprophss1 Hprophet_model".
+      iStep. iIntros "%prophs %Hprophss1 Hprophet_model".
       iDestruct (owner_agree with "Howner₁ Howner₂") as %(<- & <- & <-).
       iDestruct (front_lb_valid with "Hfront_auth Hfront_lb") as %?.
       iDestruct (inv_state_Stable with "Hstate") as "#([-> | ->] & _)"; first done.
